A/B denot_set

DenotationalLean/Denot.lean
@@ -29,3 +29,43 @@ theorem c_denot_correct :
     have ex : ∃ σ', ⟨c,σ⟩ ~~> σ' := ⟨σ', h⟩
     have _ := choose_spec ex
     grind [c_unique]
+
+def a_denot_set (a : Aexp) : Set (State × Nat) :=
+  match a with
+  | .Nat n => {(σ,n) | σ : State}
+  | .Loc l => {(σ,σ{l}) | σ : State}
+  | .Add a0 a1 => {(σ,n) | ∃ (n0 n1 : Nat) , n0 + n1 = n ∧ (σ,n0) ∈ a_denot_set a0 ∧ (σ,n1) ∈ a_denot_set a1}
+  | .Sub a0 a1 => {(σ,n) | ∃ (n0 n1 : Nat) , n0 - n1 = n ∧ (σ,n0) ∈ a_denot_set a0 ∧ (σ,n1) ∈ a_denot_set a1}
+  | .Mul a0 a1 => {(σ,n) | ∃ (n0 n1 : Nat) , n0 * n1 = n ∧ (σ,n0) ∈ a_denot_set a0 ∧ (σ,n1) ∈ a_denot_set a1}
+
+theorem a_denot_equiv :
+  ∀ (a : Aexp) (σ : State) (n : Nat) , a_denot a σ = n <-> (σ,n) ∈ a_denot_set a
+:= by
+  intro a σ
+  induction a with
+  | Nat | Loc =>
+    simp [a_denot_set, a_denot, a_eval]
+  | Add a0 a1 | Sub a0 a1 | Mul a0 a1 =>
+    simp [a_denot_set, a_denot, a_eval]
+    intro n
+    apply Iff.intro
+    . intro h
+      use a_denot a0 σ
+      use a_denot a1 σ
+      grind [a_denot]
+    . grind [a_denot]
+
+def b_denot_set (b : Bexp) : Set (State × Bool) :=
+  match b with
+  | .Bool t => {(σ,t) | σ : State}
+  | .Eq a0 a1 => {(σ,a_eval a0 σ == a_eval a1 σ) | σ : State}
+  | .Le a0 a1 => {(σ,decide (a_eval a0 σ <= a_eval a1 σ)) | σ : State}
+  | .Not b => {(σ,t) | ∃ (t' : Bool) , (t = !t') ∧ (σ,t') ∈ b_denot_set b}
+  | .And b0 b1 => {(σ,t) | ∃ (t0 t1 : Bool) , t = (t0 && t1) ∧ (σ,t0) ∈ b_denot_set b0 ∧ (σ,t1) ∈ b_denot_set b1}
+  | .Or  b0 b1 => {(σ,t) | ∃ (t0 t1 : Bool) , t = (t0 || t1) ∧ (σ,t0) ∈ b_denot_set b0 ∧ (σ,t1) ∈ b_denot_set b1}
+
+theorem b_denot_equiv :
+  ∀ (b : Bexp) (σ : State) (t : Bool) , b_denot b σ = t <-> (σ,t) ∈ b_denot_set b
+:= by
+  intro b
+  induction b <;> simp [b_denot_set, b_denot, b_eval] <;> grind [b_denot]
